Hash input strings in reader
The old s2c function allocated lots of string literals on each call, and
the same string was compared many times. Now the input string is hashed
once and compared against a few integer literals. This results in a
modest speed gain.

examples/opentheory/readerScript.sml
@@ -76,6 +76,19 @@ End
  * TODO: Maybe: hash string?
  *)
 
+Definition strh_aux_def:
+  strh_aux s a n =
+    if n ≥ strlen s then a else strh_aux s (13 * a + ORD (strsub s n)) (n + 1)
+Termination
+  WF_REL_TAC ‘measure (λ(s,a,n). strlen s - n)’
+End
+
+Definition strh_def:
+  strh s = strh_aux s 0 0
+End
+
+fun str_hash mls = rconc (EVAL “strh ^(mls)”);
+
 Definition s2c_def:
   s2c s =
     if strlen s = 0 then unknownc s else
@@ -86,41 +99,43 @@ Definition s2c_def:
           case fromString s of
             NONE => unknownc s
           | SOME i => intc i
-        else if s = «absTerm» then absTerm
-        else if s = «absThm» then absThm
-        else if s = «appTerm» then appTerm
-        else if s = «appThm» then appThm
-        else if s = «assume» then assume
-        else if s = «axiom» then axiom
-        else if s = «betaConv» then betaConv
-        else if s = «cons» then cons
-        else if s = «const» then const
-        else if s = «constTerm» then constTerm
-        else if s = «deductAntisym» then deductAntisym
-        else if s = «def» then def
-        else if s = «defineConst» then defineConst
-        else if s = «defineConstList» then defineConstList
-        else if s = «defineTypeOp» then defineTypeOp
-        else if s = «eqMp» then eqMp
-        else if s = «hdTl» then hdTl
-        else if s = «nil» then nil
-        else if s = «opType» then opType
-        else if s = «pop» then popc
-        else if s = «pragma» then pragma
-        else if s = «proveHyp» then proveHyp
-        else if s = «ref» then ref
-        else if s = «refl» then refl
-        else if s = «remove» then remove
-        else if s = «subst» then subst
-        else if s = «sym» then sym
-        else if s = «thm» then thm
-        else if s = «trans» then trans
-        else if s = «typeOp» then typeOp
-        else if s = «var» then var
-        else if s = «varTerm» then varTerm
-        else if s = «varType» then varType
-        else if s = «version» then version
-        else unknownc s
+        else
+          let h = strh s in
+            if h = ^(str_hash “«absTerm»”) then absTerm
+            else if h = ^(str_hash “«absThm»”) then absThm
+            else if h = ^(str_hash “«appTerm»”) then appTerm
+            else if h = ^(str_hash “«appThm»”) then appThm
+            else if h = ^(str_hash “«assume»”) then assume
+            else if h = ^(str_hash “«axiom»”) then axiom
+            else if h = ^(str_hash “«betaConv»”) then betaConv
+            else if h = ^(str_hash “«cons»”) then cons
+            else if h = ^(str_hash “«const»”) then const
+            else if h = ^(str_hash “«constTerm»”) then constTerm
+            else if h = ^(str_hash “«deductAntisym»”) then deductAntisym
+            else if h = ^(str_hash “«def»”) then def
+            else if h = ^(str_hash “«defineConst»”) then defineConst
+            else if h = ^(str_hash “«defineConstList»”) then defineConstList
+            else if h = ^(str_hash “«defineTypeOp»”) then defineTypeOp
+            else if h = ^(str_hash “«eqMp»”) then eqMp
+            else if h = ^(str_hash “«hdTl»”) then hdTl
+            else if h = ^(str_hash “«nil»”) then nil
+            else if h = ^(str_hash “«opType»”) then opType
+            else if h = ^(str_hash “«pop»”) then popc
+            else if h = ^(str_hash “«pragma»”) then pragma
+            else if h = ^(str_hash “«proveHyp»”) then proveHyp
+            else if h = ^(str_hash “«ref»”) then ref
+            else if h = ^(str_hash “«refl»”) then refl
+            else if h = ^(str_hash “«remove»”) then remove
+            else if h = ^(str_hash “«subst»”) then subst
+            else if h = ^(str_hash “«sym»”) then sym
+            else if h = ^(str_hash “«thm»”) then thm
+            else if h = ^(str_hash “«trans»”) then trans
+            else if h = ^(str_hash “«typeOp»”) then typeOp
+            else if h = ^(str_hash “«var»”) then var
+            else if h = ^(str_hash “«varTerm»”) then varTerm
+            else if h = ^(str_hash “«varType»”) then varType
+            else if h = ^(str_hash “«version»”) then version
+            else unknownc s
 End
 
 (*
